Publish previews: main 7b89b69a, 9 PRs, 2 unavailable
Main: 7b89b69a

Pull requests:
- PR #181: published at 7e02bb1d (9 changed variants)
- PR #185: published at b7729749 (9 changed variants)
- PR #256: published at ef4d2fc5 (9 changed variants)
- PR #286: published at 89664253 (9 changed variants)
- PR #301: published at 2818afa0 (9 changed variants)
- PR #303: published at 66999db5 (9 changed variants)
- PR #307: waiting-ci at a10822c1
- PR #319: published at 6406c730 (9 changed variants)
- PR #320: published at 0a58e0b6 (9 changed variants)
- PR #323: published at ba6bc3f1 (9 changed variants)
- PR #324: waiting-ci at c6c047f2

pr/301/head/lf/student/html/-verso-search/searchIndex_219.3010f734651144f4.js
@@ -1,0 +1,1 @@
+window.docContents[219].resolve({"/Induction/#Induction":{"contents":"\n\n\n\n\n\n\n\n\n\n\n\n\n\n\n\n\n\n","context":"Logical Foundations","header":"3. Induction: Proof by Induction","id":"/Induction/#Induction"}});
